multi-one simulation mapping in practice, compressed most mapping congruence lemmas

core/TotalMapSimulations.v
@@ -122,19 +122,21 @@ Class MultiOneNodeParamsTotalMap
     tot_one_map_msg : name -> name -> msg -> @input B1
   }.
 
+(*
 Class MultiOneNodeParamsTotalMapCongruency
  (B0 : BaseParams) (B1 : BaseParams)
  (P0 : MultiParams B0) (P1 : OneNodeParams B1)
- (P : MultiOneNodeParamsTotalMap P0 B1) :=
+ (P : MultiOneNodeParamsTotalMap P0 B1) (n : name) :=
  {
-   tot_init_eq : forall n, tot_one_map_data (init_handlers n) = init ;
-   tot_net_handlers_handler_eq : forall me src m st out st' ps out',
-     net_handlers me src m st = (out, st', ps) ->
-     handler (tot_one_map_msg me src m) (tot_one_map_data st) = (out', tot_one_map_data st') ;
-   tot_input_handlers_handler_eq : forall me inp st out st' ps out',
-     input_handlers me inp st = (out, st', ps) ->
-     handler (tot_one_map_input me inp) (tot_one_map_data st) = (out', tot_one_map_data st')
+   tot_init_eq : tot_one_map_data (init_handlers n) = init ;
+   tot_net_handlers_handler_eq : forall src m st out st' ps out',
+     net_handlers n src m st = (out, st', ps) ->
+     handler (tot_one_map_msg n src m) (tot_one_map_data st) = (out', tot_one_map_data st') ;
+   tot_input_handlers_handler_eq : forall inp st out st' ps out',
+     input_handlers n inp st = (out, st', ps) ->
+     handler (tot_one_map_input n inp) (tot_one_map_data st) = (out', tot_one_map_data st')
  }.
+*)
 
 Section TotalMapBijective.
 
@@ -1422,56 +1424,86 @@ Qed.
 
 Context {one_snd : OneNodeParams base_snd}.
 Context {multi_fst_snd : MultiOneNodeParamsTotalMap multi_fst base_snd}.
-Context {multi_one : MultiOneNodeParamsTotalMapCongruency one_snd multi_fst_snd}.
+(*Context {n} {multi_one : MultiOneNodeParamsTotalMapCongruency one_snd multi_fst_snd n}.*)
+
+Section OneMapped.
+
+Context {n : @name _ multi_fst}.
+
+Hypothesis tot_init_eq : tot_one_map_data (init_handlers n) = init.
+
+Definition tot_net_handlers_handler_eq (f : @name _ multi_fst -> @data base_fst) :=
+  forall src m out st' ps out', 
+    net_handlers n src m (f n) = (out, st', ps) -> 
+    handler (tot_one_map_msg n src m) (tot_one_map_data (f n)) = (out', tot_one_map_data st').
+
+Definition tot_input_handlers_handler_eq (f : @name _ multi_fst -> @data base_fst) :=
+  forall inp out st' ps out',
+    input_handlers n inp (f n) = (out, st', ps) ->
+    handler (tot_one_map_input n inp) (tot_one_map_data (f n)) = (out', tot_one_map_data st').
 
 Theorem step_m_tot_one_mapped_simulation_1 :
   forall net net' tr,
+    tot_net_handlers_handler_eq net.(nwState) ->
+    tot_input_handlers_handler_eq net.(nwState) ->
     @step_m _ multi_fst net net' tr ->
-    forall n, net.(nwState) n = net'.(nwState) n \/
+    net.(nwState) n = net'.(nwState) n \/
     exists tr', @step_1 _ one_snd (tot_one_map_data (net.(nwState) n)) (tot_one_map_data (net'.(nwState) n)) tr'.
 Proof.
-move => net net' tr.
-case => {net net' tr}.
-- move => net net' p ms ms' out d l H_eq H_hnd H_eq' n.
+move => net net' tr H_eq_net H_eq_inp H_st.
+case: H_st H_eq_net H_eq_inp => {net net' tr}.
+- move => net net' p ms ms' out d l H_eq H_hnd H_eq' H_eq_net H_eq_inp.
   rewrite H_eq' /= /update.
   break_if; last by left.
   right.
   rewrite -e in H_hnd.
   case H_h: (handler (tot_one_map_msg (pDst p) (pSrc p) (pBody p)) (tot_one_map_data (nwState net (pDst p)))) => [out' st'].
-  apply (tot_net_handlers_handler_eq _ _ _ _ out') in H_hnd.
+  apply (H_eq_net _ _ _ _ _ out') in H_hnd.
   exists [(tot_one_map_msg (pDst p) (pSrc p) (pBody p), out')].
   apply: S1T_deliver => //.
   by rewrite -H_hnd e.
-- move => h net net' out inp d ps H_hnd H_eq n.
+- move => h net net' out inp d ps H_hnd H_eq H_eq_net H_eq_inp.
   rewrite H_eq /= /update.
   break_if; last by left.
   right.
   rewrite e.
   case (handler (tot_one_map_input h inp) (tot_one_map_data (nwState net h))) => [out' st'].
-  apply (tot_input_handlers_handler_eq _ _ _ out') in H_hnd.
+  rewrite -e in H_hnd.
+  apply (H_eq_inp _ _ _ _ out') in H_hnd.
+  rewrite e in H_hnd.
   exists [((tot_one_map_input h inp), out')].
   exact: S1T_deliver.
 Qed.
 
+Hypothesis step_m_star_tot_net_handlers_eq :
+  forall net tr,
+    @step_m_star _ multi_fst step_m_init net tr ->
+    tot_net_handlers_handler_eq net.(nwState).
+
+Hypothesis step_m_star_tot_input_handlers_eq :
+  forall net tr,
+    @step_m_star _ multi_fst step_m_init net tr ->
+    tot_input_handlers_handler_eq net.(nwState).
+
 Corollary step_m_tot_one_mapped_simulation_star_1 :
   forall net tr,
     @step_m_star _ multi_fst step_m_init net tr ->
-    forall n, exists tr', @step_1_star _ one_snd init (tot_one_map_data (net.(nwState) n)) tr'.
+    exists tr', @step_1_star _ one_snd init (tot_one_map_data (net.(nwState) n)) tr'.
 Proof.
 move => net tr H_st.
-remember step_m_init as y in *.
+remember step_m_init as y in H_st.
 move: Heqy.
 induction H_st using refl_trans_1n_trace_n1_ind => H_init /=.
-  move => n.
   rewrite H_init /step_m_init /=.
   rewrite tot_init_eq.
   exists [].
   exact: RT1nTBase.
 concludes.
 repeat find_rewrite.
-move => n.
-have H_st' := step_m_tot_one_mapped_simulation_1 H n.
-have [tr' H_st] := IHH_st1 n.
+have H_eq_net := step_m_star_tot_net_handlers_eq H_st1.
+have H_eq_inp := step_m_star_tot_input_handlers_eq H_st1.
+have H_st' := step_m_tot_one_mapped_simulation_1 H_eq_net H_eq_inp H.
+have [tr' H_st] := IHH_st1.
 case: H_st' => H_st'.
   rewrite -H_st'.
   by exists tr'.
@@ -1486,18 +1518,20 @@ Qed.
 
 Theorem step_o_f_tot_one_mapped_simulation_1 :
   forall net net' failed failed' tr,
+    tot_net_handlers_handler_eq net.(onwState) ->
+    tot_input_handlers_handler_eq net.(onwState) ->
     @step_o_f _ _ overlay_fst fail_msg_fst (failed, net) (failed', net') tr ->
-    forall n, net.(onwState) n = net'.(onwState) n \/
+    net.(onwState) n = net'.(onwState) n \/
     exists tr', @step_1 _ one_snd (tot_one_map_data (net.(onwState) n)) (tot_one_map_data (net'.(onwState) n)) tr'.
 Proof.
-move => net net' failed failed' tr H_step n.
+move => net net' failed failed' tr H_eq_net H_eq_inp H_step.
 invcs H_step.
 - rewrite /update'.
   break_if; last by left.
   right.
   rewrite -e in H6.
   case H_h: (handler (tot_one_map_msg to from m) (tot_one_map_data (onwState net n))) => [out' st'].
-  apply (tot_net_handlers_handler_eq _ _ _ _ out') in H6.
+  apply (H_eq_net _ _ _ _ _ out') in H6.
   exists [(tot_one_map_msg to from m, out')].
   apply: S1T_deliver => //.
   by rewrite -H6 e.
@@ -1506,25 +1540,36 @@ invcs H_step.
   right.
   rewrite e.
   case (handler (tot_one_map_input h inp) (tot_one_map_data (onwState net h))) => [out' st'].
-  apply (tot_input_handlers_handler_eq _ _ _ out') in H5.
+  rewrite -e in H5.
+  apply (H_eq_inp _ _ _ _ out') in H5.
+  rewrite e in H5.
   exists [((tot_one_map_input h inp), out')].
   exact: S1T_deliver.
 - by left.
 Qed.
 
+Hypothesis step_o_f_star_tot_net_handlers_eq :
+  forall net failed tr,
+    @step_o_f_star _ _ overlay_fst fail_msg_fst step_o_f_init (failed, net) tr ->
+    tot_net_handlers_handler_eq net.(onwState).
+
+Hypothesis step_o_f_star_tot_input_handlers_eq :
+  forall net failed tr,
+    @step_o_f_star _  _ overlay_fst fail_msg_fst step_o_f_init (failed, net) tr ->
+    tot_input_handlers_handler_eq net.(onwState).
+
 Corollary step_o_f_tot_one_mapped_simulation_star_1 :
   forall net failed tr,
     @step_o_f_star _ _ overlay_fst fail_msg_fst step_o_f_init (failed, net) tr ->
-    forall n, exists tr', @step_1_star _ one_snd init (tot_one_map_data (net.(onwState) n)) tr'.
+    exists tr', @step_1_star _ one_snd init (tot_one_map_data (net.(onwState) n)) tr'.
 Proof.
 move => net failed tr H_st.
-remember step_o_f_init as y in *.
+remember step_o_f_init as y in H_st.
 have H_eq_n: net = snd (failed, net) by [].
 rewrite H_eq_n {H_eq_n}.
 move: Heqy.
 induction H_st using refl_trans_1n_trace_n1_ind => H_init /=.
   rewrite H_init /=.
-  move => n.
   exists [].
   rewrite tot_init_eq.
   exact: RT1nTBase.
@@ -1533,13 +1578,15 @@ rewrite H_init {H_init x} in H_st1 H_st2.
 case: x' H IHH_st1 H_st1 => failed' net'.
 case: x'' H_st2 => failed'' net''.
 rewrite /=.
-move => H_step2 H IHH_step1 H_step1 n.
-have H_stt := step_o_f_tot_one_mapped_simulation_1 H n.
+move => H_step2 H IHH_step1 H_step1.
+have H_eq_net := step_o_f_star_tot_net_handlers_eq H_step1.
+have H_eq_inp := step_o_f_star_tot_input_handlers_eq H_step1.
+have H_stt := step_o_f_tot_one_mapped_simulation_1 H_eq_net H_eq_inp H.
 case: H_stt => H_stt.
   rewrite -H_stt.
-  have [tr' H_star] := IHH_step1 n.
+  have [tr' H_star] := IHH_step1.
   by exists tr'.
-have [tr' H_star] := IHH_step1 n.
+have [tr' H_star] := IHH_step1.
 have [tr'' H_step] := H_stt.
 exists (tr' ++ tr'').
 have H_trans := refl_trans_1n_trace_trans H_star.
@@ -1548,6 +1595,8 @@ have ->: tr'' = tr'' ++ [] by rewrite -app_nil_end.
 apply RT1nTStep with (x' := (tot_one_map_data (onwState net'' n))) => //.
 exact: RT1nTBase.
 Qed.
+
+End OneMapped.
 
 (*
 Context {new_msg_fst : NewMsgParams multi_fst}.
