systems/AggregatorStatic.v
@@ -1,0 +1,325 @@
+Require Import Verdi.
+Require Import StateMachineHandlerMonad.
+Require Import NameOverlay.
+
+Require Import UpdateLemmas.
+Local Arguments update {_} {_} {_} _ _ _ _ : simpl never.
+
+Require Import mathcomp.ssreflect.ssreflect.
+Require Import mathcomp.ssreflect.ssrbool.
+Require Import mathcomp.ssreflect.eqtype.
+Require Import mathcomp.ssreflect.fintype.
+Require Import mathcomp.ssreflect.finset.
+Require Import mathcomp.fingroup.fingroup.
+
+Require Import Orders.
+Require Import MSetFacts.
+Require Import MSetProperties.
+
+Require Import Sumbool.
+
+Require Import AggregationDefinitions.
+Require Import AggregationAux.
+
+Require Import AAC_tactics.AAC.
+
+Module OneAggregator (Import NT : NameType)
+ (NOT : NameOrderedType NT) (NSet : MSetInterface.S with Module E := NOT) 
+ (NOTC : NameOrderedTypeCompat NT) (NMap : FMapInterface.S with Module E := NOTC) 
+ (Import CFG : CommutativeFinGroup) (Import ANT : AdjacentNameType NT).
+
+Module A := Adjacency NT NOT NSet ANT.
+Import A.
+
+Module AX := AAux NT NOT NSet NOTC NMap CFG ANT.
+Import AX.AD.
+Import AX.
+
+Import GroupScope.
+
+Module NSetFacts := Facts NSet.
+Module NSetProps := Properties NSet.
+Module NSetOrdProps := OrdProperties NSet.
+
+Require Import FMapFacts.
+Module NMapFacts := Facts NMap.
+
+Inductive Input : Type :=
+| Aggregate : name -> m -> Input
+| Fail : name -> Input
+| Local : m -> Input
+| SendAggregate : name -> Input
+| AggregateRequest : Input.
+
+Definition Input_eq_dec : forall x y : Input, {x = y} + {x <> y}.
+decide equality.
+- exact: m_eq_dec.
+- exact: name_eq_dec.
+- exact: name_eq_dec.
+- exact: m_eq_dec.
+- exact: name_eq_dec.
+Defined.
+
+Inductive Output : Type :=
+| AggregateResponse : m -> Output
+| Unit : Output.
+
+Definition Output_eq_dec : forall x y : Output, {x = y} + {x <> y}.
+decide equality.
+exact: m_eq_dec.
+Defined.
+
+Record Data := mkData { 
+  local : m ; 
+  aggregate : m ; 
+  adjacent : NS ; 
+  sent : NM ; 
+  received : NM 
+}.
+
+Definition InitData (n : name) :=
+  {| local := 1 ;
+     aggregate := 1 ;
+     adjacent := adjacency n nodes ;
+     sent := init_map (adjacency n nodes) ;
+     received := init_map (adjacency n nodes) |}.
+
+Definition Handler (S : Type) := GenHandler1 S Output.
+
+Definition IOHandler (i : Input) : Handler Data :=
+st <- get ;;
+match i with
+| Aggregate src m_inp =>  
+  when (NSet.mem src st.(adjacent))
+  (match NMap.find src st.(received) with
+  | None => nop
+  | Some m_src => 
+    put {| local := st.(local) ;
+           aggregate := st.(aggregate) * m_inp ;
+           adjacent := st.(adjacent) ;
+           sent := st.(sent) ;
+           received := NMap.add src (m_src * m_inp) st.(received) |}                                                           
+  end) ;;
+  write_output Unit
+| Fail src =>
+  when (NSet.mem src st.(adjacent))
+  (match NMap.find src st.(sent), NMap.find src st.(received) with
+  | Some m_snt, Some m_rcd =>    
+    put {| local := st.(local) ;
+           aggregate := st.(aggregate) * m_snt * (m_rcd)^-1 ;
+           adjacent := NSet.remove src st.(adjacent) ;
+           sent := NMap.remove src st.(sent) ;
+           received := NMap.remove src st.(received) |}           
+  | _, _ => nop    
+  end) ;;
+  write_output Unit
+| Local m_inp =>
+  put {| local := m_inp ;
+         aggregate := st.(aggregate) * m_inp * st.(local)^-1 ;
+         adjacent := st.(adjacent) ;
+         sent := st.(sent) ;
+         received := st.(received) |} ;;
+  write_output Unit
+| AggregateRequest =>  
+  write_output (AggregateResponse st.(aggregate))
+| SendAggregate dst =>
+  when (NSet.mem dst st.(adjacent) && sumbool_not _ _ (m_eq_dec st.(aggregate) 1))
+  (match NMap.find dst st.(sent) with
+   | None => nop
+   | Some m_dst =>        
+     put {| local := st.(local) ;
+            aggregate := 1 ;
+            adjacent := st.(adjacent) ;
+            sent := NMap.add dst (m_dst * st.(aggregate)) st.(sent) ;
+            received := st.(received) |}
+   end) ;;
+  write_output Unit
+end.
+
+Instance Aggregator_BaseParams : BaseParams := 
+  {
+    data := Data ;
+    input := Input ;
+    output := Output
+  }.
+
+Instance Aggregator_OneNodeParams (n : name) : OneNodeParams Aggregator_BaseParams :=
+  {
+    init := InitData n;
+    handler := fun i d => runGenHandler1 d (IOHandler i) 
+  }.
+
+Lemma IOHandler_cases :
+  forall i st out st',
+      IOHandler i st = (out, st') ->
+      (exists m_inp m_src src, i = Aggregate src m_inp /\ NSet.In src st.(adjacent) /\ NMap.find src st.(received) = Some m_src /\
+       st'.(local) = st.(local) /\
+       st'.(aggregate) = st.(aggregate) * m_inp /\
+       st'.(adjacent) = st.(adjacent) /\
+       st'.(sent) = st.(sent) /\     
+       st'.(received) = NMap.add src (m_src * m_inp) st.(received) /\
+       out = Unit) \/
+      (exists m_inp src, i = Aggregate src m_inp /\ NSet.In src st.(adjacent) /\ NMap.find src st.(received) = None /\ 
+       st' = st /\ out = Unit) \/
+      (exists m_inp src, i = Aggregate src m_inp /\ ~ NSet.In src st.(adjacent) /\
+       st' = st /\ out = Unit) \/
+      (exists m_snt m_rcd src, i = Fail src /\ NSet.In src st.(adjacent) /\ NMap.find src st.(sent) = Some m_snt /\ NMap.find src st.(received) = Some m_rcd /\
+       st'.(local) = st.(local) /\ 
+       st'.(aggregate) = st.(aggregate) * m_snt * (m_rcd)^-1 /\
+       st'.(adjacent) = NSet.remove src st.(adjacent) /\
+       st'.(sent) = NMap.remove src st.(sent) /\
+       st'.(received) = NMap.remove src st.(received) /\
+       out = Unit) \/
+      (exists src, i = Fail src /\ NSet.In src st.(adjacent) /\ NMap.find src st.(received) = None /\
+       st' = st /\ out = Unit) \/
+      (exists src, i = Fail src /\ NSet.In src st.(adjacent) /\ NMap.find src st.(sent) = None /\
+       st' = st /\ out = Unit) \/
+      (exists src, i = Fail src /\ ~ NSet.In src st.(adjacent) /\
+       st' = st /\ out = Unit) \/
+      (exists m_inp, i = Local m_inp /\ 
+       st'.(local) = m_inp /\ 
+       st'.(aggregate) = st.(aggregate) * m_inp * st.(local)^-1 /\ 
+       st'.(adjacent) = st.(adjacent) /\
+       st'.(sent) = st.(sent) /\
+       st'.(received) = st.(received) /\
+       out = Unit) \/
+      (exists dst m', i = SendAggregate dst /\ NSet.In dst st.(adjacent) /\ st.(aggregate) <> 1 /\ NMap.find dst st.(sent) = Some m' /\
+         st'.(local) = st.(local) /\ 
+         st'.(aggregate) = 1 /\
+         st'.(adjacent) = st.(adjacent) /\
+         st'.(sent) = NMap.add dst (m' * st.(aggregate)) st.(sent) /\
+         st'.(received) = st.(received) /\
+         out = Unit) \/
+      (exists dst, i = SendAggregate dst /\ NSet.In dst st.(adjacent) /\ st.(aggregate) <> 1 /\ NMap.find dst st.(sent) = None /\
+         st' = st /\
+         out = Unit) \/
+      (exists dst, i = SendAggregate dst /\ ~ NSet.In dst st.(adjacent) /\ 
+         st' = st /\ 
+         out = Unit) \/
+      (exists dst, i = SendAggregate dst /\ st.(aggregate) = 1 /\
+         st' = st /\ 
+         out = Unit) \/
+      (i = AggregateRequest /\ st' = st /\ out = AggregateResponse (aggregate st)).
+Proof.
+move => i st out st'.
+rewrite /IOHandler.
+case: i => [src m_inp|src|m_inp|dst|]; monad_unfold.
+- move => H_eq.
+  repeat break_match; repeat tuple_inversion.
+  * find_apply_lem_hyp NSetFacts.mem_2.
+    left => /=.
+    by exists m_inp; exists a; exists src.
+  * find_apply_lem_hyp NSetFacts.mem_2.
+    right; left => /=.
+    by exists m_inp; exists src.
+  * have H_ins: ~ NSet.In src st'.(adjacent) by move => H_ins; find_apply_lem_hyp NSetFacts.mem_1; eauto.
+    right; right; left.
+    by exists m_inp; exists src.
+- move => H_eq.
+  repeat break_match; repeat tuple_inversion.
+  * find_apply_lem_hyp NSetFacts.mem_2.
+    right; right; right; left => /=.
+    by exists a; exists a0; exists src.
+  * find_apply_lem_hyp NSetFacts.mem_2.
+    right; right; right; right; left => /=.
+    by exists src.
+  * find_apply_lem_hyp NSetFacts.mem_2.
+    right; right; right; right; right; left => /=.
+    by exists src.
+  * have H_ins: ~ NSet.In src st'.(adjacent) by move => H_ins; find_apply_lem_hyp NSetFacts.mem_1; eauto.
+    right; right; right; right; right; right; left => /=.
+    by exists src.
+- move => H_eq.
+  repeat tuple_inversion.
+  right; right; right; right; right; right; right; left => /=.
+  by exists m_inp.
+- move => H_eq.
+  repeat break_let; break_if; first (break_let; break_match).
+  * move/andP: Heqb => /= [H_mem H_neq].
+    repeat tuple_inversion.
+    rewrite /sumbool_not in H_neq.
+    break_match => //.
+    find_apply_lem_hyp NSetFacts.mem_2.
+    right; right; right; right; right; right; right; right; left => /=.
+    by exists dst; exists a.
+  * move/andP: Heqb => /= [H_mem H_neq].
+    repeat tuple_inversion.
+    rewrite /sumbool_not in H_neq.
+    break_match => //.
+    find_apply_lem_hyp NSetFacts.mem_2.
+    right; right; right; right; right; right; right; right; right; left => /=.
+    by exists dst.
+  * move/nandP: Heqb => /= Heqb.
+    repeat tuple_inversion.
+    break_or_hyp.
+      move/negP: H => H.
+      have H_ins: ~ NSet.In dst st'.(adjacent) by move => H_ins; find_apply_lem_hyp NSetFacts.mem_1.
+      right; right; right; right; right; right; right; right; right; right; left => /=.
+      by exists dst.
+    unfold sumbool_not in *.
+    break_match => //.
+    right; right; right; right; right; right; right; right; right; right; right; left => /=.
+    by exists dst.
+- move => H_eq.
+  tuple_inversion.
+  by right; right; right; right; right; right; right; right; right; right; right; right.
+Qed.
+
+Ltac io_handler_cases := 
+  find_apply_lem_hyp IOHandler_cases; 
+  intuition idtac; try break_exists; 
+  intuition idtac; subst; 
+  repeat find_rewrite.
+
+Instance AggregationData_Data : AggregationData Data :=
+  {
+    aggr_local := local ;
+    aggr_aggregate := aggregate ;
+    aggr_adjacent := adjacent ;
+    aggr_sent := sent ;
+    aggr_received := received
+  }.
+
+Lemma Aggregator_conserves_node_mass : 
+ forall n st tr, @step_1_star _ (Aggregator_OneNodeParams n) (@init _ (Aggregator_OneNodeParams n))  st tr ->
+  conserves_node_mass st.
+Proof.
+move => n st tr H_st.
+remember init as y in *.
+move: Heqy.
+induction H_st using refl_trans_1n_trace_n1_ind => H_init; first by rewrite H_init /conserves_node_mass /InitData; gsimpl.
+concludes.
+match goal with
+| [ H : step_1 _ _ _ |- _ ] => invc H
+end; simpl.
+rewrite /handler /= /runGenHandler1 /= in H0.
+io_handler_cases; unfold conserves_node_mass in *; simpl in * => //.
+- repeat find_rewrite.
+  rewrite sumM_add_map //; gsimpl.
+  set m1 := aggregate _.
+  set m2 := sumM _ _.
+  set m3 := sumM _ _.
+  suff H_suff: m1 * x * m2 * x^-1 * m3^-1 = m1 * m2 * m3^-1 * (x * x^-1) by rewrite H_suff; gsimpl.
+  by aac_reflexivity.
+- repeat find_rewrite.
+  rewrite (sumM_remove_remove H H1) (sumM_remove_remove H H2); gsimpl.
+  set m1 := aggregate _.
+  set m2 := sumM _ _.
+  set m3 := sumM _ _.
+  suff H_suff: m1 * x * x0^-1 * m2 * x^-1 * x0 * m3^-1 = m1 * m2 * m3^-1 * (x * x^-1) * (x0 * x0^-1) by rewrite H_suff; gsimpl.
+  by aac_reflexivity.
+- repeat find_rewrite.
+  gsimpl.
+  set m0 := local _.
+  set m1 := aggregate _.
+  set m2 := sumM _ _.
+  set m3 := sumM _ _.
+  suff H_suff: m1 * m0 * m2 * m3^-1 * m1^-1 * m3 * m2^-1 = m0 * (m1 * m1^-1) * (m2 * m2^-1) * (m3 * m3^-1) by rewrite H_suff; gsimpl.
+  by aac_reflexivity.
+- repeat find_rewrite.
+  rewrite sumM_add_map //.
+  gsimpl.
+  by aac_reflexivity.
+Qed.
+
+End OneAggregator.
